prove inductive table to formal table

Clean/Table/Inductive.lean
@@ -6,7 +6,7 @@ Assignment of cells is handled in the background, which simplifies reasoning abo
 
 The common `k=2` case gets its own special definition.
 -/
-import Clean.Table.Basic
+import Clean.Table.Theorems
 import Clean.Gadgets.Equality
 
 /--
@@ -14,7 +14,7 @@ In the case of two-row windows, an `InductiveTable` is basically a `FormalCircui
 - with the same input and output types
 - with an extra input to the spec: the current (input) row number
 - with assumptions replaced by the spec on the previous row
-- with input offset hard-coded to zero
+- with input offset hard-coded to `size Row`
 -/
 structure InductiveTable (F : Type) [Field F] (Row : Type → Type) [LawfulProvableType Row] where
   main : Var Row F → Circuit F (Var Row F)
@@ -24,21 +24,21 @@ structure InductiveTable (F : Type) [Field F] (Row : Type → Type) [LawfulProva
     -- for all rows
     ∀ (input_var : Var Row F) (input : Row F), eval env input_var = input →
     -- if the constraints hold
-    Circuit.constraints_hold.soundness env (main input_var |>.operations) →
+    Circuit.constraints_hold.soundness env (main input_var |>.operations (size Row)) →
     -- and assuming the spec on the input row
     spec row_index input →
     -- we can conclude the spec on the output row
-    spec (row_index + 1) (eval env (main input_var |>.output))
+    spec (row_index + 1) (eval env (main input_var |>.output (size Row)))
 
   completeness : ∀ (row_index : ℕ) (env : Environment F),
     -- for all rows
     ∀ (input_var : Var Row F) (input : Row F), eval env input_var = input →
     -- when using honest-prover witnesses
-    env.uses_local_witnesses_completeness 0 (main input_var |>.operations) →
+    env.uses_local_witnesses_completeness (size Row) (main input_var |>.operations (size Row)) →
     -- and assuming the spec on the input row
     spec row_index input →
     -- the constraints hold
-    Circuit.constraints_hold.completeness env (main input_var |>.operations)
+    Circuit.constraints_hold.completeness env (main input_var |>.operations (size Row))
 
   subcircuits_consistent : ∀ var, ((main var).operations).subcircuits_consistent 0
     := by intros; and_intros <;> (
@@ -54,10 +54,10 @@ def tableSpec (table : InductiveTable F Row) {N : ℕ} (trace : TraceOfLength F 
 
 def inductiveConstraint (table : InductiveTable F Row) : TableConstraint 2 Row F Unit := do
   let input ← get_curr_row
-  let output ← get_next_row
-  let output' ← table.main input
+  let output ← table.main input
+  let output' ← get_next_row
   -- TODO make this more efficient by assigning variables as long as they don't come from the input
-  assert_equals output output'
+  assert_equals output' output
 
 def equalityConstraint (target : Row F) : SingleRowConstraint Row F := do
   let actual ← get_curr_row
@@ -71,20 +71,98 @@ def tableConstraints (table : InductiveTable F Row) (input output: Row F) :
     -- .Boundary (N - 1) (equalityConstraint output)
   ]
 
-theorem tableSoundness : ∀ (table : InductiveTable F Row) (input output: Row F)
-  (N : ℕ) (trace: TraceOfLength F Row N) (env: ℕ → ℕ → Environment F),
+theorem tableSoundness (table : InductiveTable F Row) (input output: Row F)
+  (N : ℕ) (trace: TraceOfLength F Row N) (env: ℕ → ℕ → Environment F) :
+  table.spec 0 input →
   table_constraints_hold (table.tableConstraints input output) trace env →
     table.tableSpec trace := by
-  sorry
+  intro input_spec
+  simp only [table_norm, tableConstraints, tableSpec]
+  induction' trace.val using Trace.everyRowTwoRowsInduction
+  case zero => intro; trivial
 
-def toFormal (table : InductiveTable F Row) (input output: Row F) : FormalTable F Row where
+  case one first_row =>
+    intro constraints
+    simp only [table_norm, tableConstraints, List.size_toArray, List.length_nil, List.push_toArray, List.nil_append,
+      List.length_cons, zero_add, List.cons_append, reduceIte, and_true] at constraints
+    set env' := window_env (equalityConstraint input) ⟨<+> +> first_row, _⟩ (env 1 0)
+    simp only [table_norm, equalityConstraint, circuit_norm] at constraints
+    simp only [table_norm, and_true]
+    have h_env i (hi : i < size Row) : (to_elements first_row)[i] = env'.get i := by
+      have h_env' : env' = window_env (equalityConstraint input) ⟨<+> +> first_row, _⟩ (env 1 0) := rfl
+      simp only [window_env, table_assignment_norm, equalityConstraint, circuit_norm] at h_env'
+      simp [h_env', hi, Vector.getElem_mapFinRange, Trace.getLeFromBottom, _root_.Row.get, Vector.get_eq,
+        Vector.mapRange_zero, Vector.append_empty]
+    have input_eq : first_row = input := by
+      rw [LawfulProvableType.ext_iff]
+      intro i hi
+      rw [h_env i hi, ←constraints, LawfulProvableType.eval_var_from_offset,
+        LawfulProvableType.to_elements_from_elements, Vector.getElem_mapRange, zero_add]
+    rw [input_eq]
+    exact input_spec
+
+  case more curr next rest ih1 ih2 =>
+    simp only [table_norm, tableConstraints, List.size_toArray, List.length_nil, List.push_toArray,
+      List.nil_append, List.length_cons, zero_add, List.cons_append, Nat.add_eq_zero, one_ne_zero,
+      and_false, reduceIte] at ih1 ih2 ⊢
+    intro ⟨ constraints, h_rest ⟩
+    specialize ih2 h_rest
+    have spec_previous : table.spec rest.len curr := by simp [ih2]
+    simp only [ih2, and_self, and_true]
+    clear ih1 ih2
+    set env' := window_env table.inductiveConstraint ⟨<+> +> curr +> next, _⟩ (env 0 (rest.len + 1))
+    simp only [table_norm, circuit_norm, inductiveConstraint] at constraints
+    obtain ⟨ main_constraints, output_eq ⟩ := constraints
+    have h_env' : env' = window_env table.inductiveConstraint ⟨<+> +> curr +> next, _⟩ (env 0 (rest.len + 1)) := rfl
+    simp only [window_env, table_assignment_norm, inductiveConstraint, circuit_norm] at h_env'
+    simp only [zero_add, Nat.add_zero, Fin.isValue, PNat.val_ofNat, Nat.reduceAdd,
+      Nat.add_one_sub_one] at h_env'
+    set curr_var := var_from_offset Row 0
+    set main_ops : Operations F := (table.main (var_from_offset Row 0) (size Row)).2
+    set s := size Row
+    set t := main_ops.local_length
+
+    have h_env_input i (hi : i < s) : (to_elements curr)[i] = env'.get i := by
+      have hi' : i < s + t + s := by linarith
+      have hi'' : i < 0 + s := by linarith
+      have hi''' : i < 0 + s + t := by linarith
+      rw [h_env']
+      simp only [main_ops, s, t, hi', hi'', hi''', table_assignment_norm, inductiveConstraint, circuit_norm, reduceDIte,
+        Vector.mapRange_zero, Vector.empty_append, Vector.append_empty, Vector.getElem_append]
+
+    have h_env_output i (hi : i < s) : (to_elements next)[i] = env'.get (i + s + t) := by
+      have hi' : i + s + t < s + t + s := by linarith
+      have hi'' : ¬(i + s + t < 0 + s) := by linarith
+      have hi''' : ¬(i + s + t < 0 + s + t) := by linarith
+      rw [h_env']
+      simp only [main_ops, hi', hi'', hi''', s, t, table_assignment_norm, inductiveConstraint, circuit_norm, reduceDIte,
+        Vector.mapRange_zero, Vector.empty_append, Vector.append_empty, Vector.getElem_append]
+      simp +arith [add_assoc]
+
+    have input_eq : eval env' curr_var = curr := by
+      rw [LawfulProvableType.ext_iff]
+      intro i hi
+      rw [h_env_input i hi, LawfulProvableType.eval_var_from_offset,
+        LawfulProvableType.to_elements_from_elements, Vector.getElem_mapRange, zero_add]
+
+    have next_eq : eval env' (var_from_offset Row (size Row + main_ops.local_length)) = next := by
+      rw [LawfulProvableType.ext_iff]
+      intro i hi
+      rw [h_env_output i hi, LawfulProvableType.eval_var_from_offset,
+        LawfulProvableType.to_elements_from_elements, Vector.getElem_mapRange, add_comm _ i, add_assoc]
+
+    have h_soundness := table.soundness rest.len env' curr_var curr input_eq main_constraints spec_previous
+    rw [←output_eq, next_eq] at h_soundness
+    exact h_soundness
+
+def toFormal (table : InductiveTable F Row) (input output: Row F) (h_input : table.spec 0 input) : FormalTable F Row where
   constraints := table.tableConstraints input output
   spec := table.tableSpec
   soundness := by
-    simp only [true_implies]
-    exact table.tableSoundness input output
+    intro N trace env _ constraints
+    exact table.tableSoundness input output _ _ _ h_input constraints
   offset_consistent := by
     simp +arith [List.Forall, tableConstraints, inductiveConstraint, equalityConstraint,
-      table_assignment_norm, circuit_norm, assignment_from_circuit_offset]
+      table_assignment_norm, circuit_norm, CellAssignment.assignment_from_circuit_offset]
 
 end InductiveTable
